James C - clean up stack language a bit

Stack/StackLanguage.thy
@@ -16,9 +16,15 @@ datatype stack_instruction =
 | Return
 | Print
 
-type_synonym stack_program = 
-  "function_name \<rightharpoonup> nat \<times> nat \<times> stack_instruction list \<times> 
-    (code_label \<rightharpoonup> stack_instruction list \<times> code_label)"
+type_synonym stack_code_block = "stack_instruction list \<times> code_label"
+
+record stack_function_def =
+  arity :: nat
+  local_count :: nat
+  main_code :: stack_code_block
+  other_code :: "code_label \<rightharpoonup> stack_code_block"
+  
+type_synonym stack_program = "function_name \<rightharpoonup> stack_function_def"
 
 datatype stack_value =
   IntV int
@@ -29,63 +35,73 @@ record frame =
   arguments :: "stack_value list"
   locals :: "stack_value list"
   saved_stack :: "stack_value list"
+  saved_code :: stack_code_block
 
-type_synonym stack_state = 
-  "stack_value list \<times> frame list \<times> stack_instruction list \<times> code_label \<times> output" 
-  (* \<sigma>, \<phi>, \<pi>, s, \<omega> *)
+type_synonym stack_state = "stack_value list \<times> frame list \<times> stack_code_block \<times> output" 
+  (* \<sigma>, \<phi>, \<pi>, \<omega> *)
 
 inductive eval_stack :: "stack_program \<Rightarrow> stack_state \<Rightarrow> stack_state \<Rightarrow> bool" where
-  evs_jump [simp]: "\<Pi> (frame.name f) = Some (a, l, \<pi>', \<Phi>) \<Longrightarrow> \<Phi> s = Some (\<pi>, s') \<Longrightarrow> 
-    eval_stack \<Pi> ([], f # \<phi>, [], s, \<omega>) ([], f # \<phi>, \<pi>, s', \<omega>)"
-| evs_add [simp]: "eval_stack \<Pi> (IntV i1 # IntV i2 # \<sigma>, \<phi>, Add # \<pi>, s, \<omega>) 
-    (IntV (i1 + i2) # \<sigma>, \<phi>, \<pi>, s, \<omega>)"
-| evs_sub [simp]: "eval_stack \<Pi> (IntV i1 # IntV i2 # \<sigma>, \<phi>, Sub # \<pi>, s, \<omega>) 
-    (IntV (i2 - i1) # \<sigma>, \<phi>, \<pi>, s, \<omega>)"
-| evs_neg [simp]: "eval_stack \<Pi> (IntV i1 # \<sigma>, \<phi>, Neg # \<pi>, s, \<omega>) (IntV (-i1) # \<sigma>, \<phi>, \<pi>, s, \<omega>)"
-| evs_eq [simp]: "eval_stack \<Pi> (IntV i1 # IntV i2 # \<sigma>, \<phi>, Eq # \<pi>, s, \<omega>) 
-    (Bool (i2 = i1) # \<sigma>, \<phi>, \<pi>, s, \<omega>)"
-| evs_gt [simp]: "eval_stack \<Pi> (IntV i1 # IntV i2 # \<sigma>, \<phi>, Gt # \<pi>, s, \<omega>) 
-    (Bool (i2 > i1) # \<sigma>, \<phi>, \<pi>, s, \<omega>)"
-| evs_lt [simp]: "eval_stack \<Pi> (IntV i1 # IntV i2 # \<sigma>, \<phi>, Lt # \<pi>, s, \<omega>) 
-    (Bool (i2 < i1) # \<sigma>, \<phi>, \<pi>, s, \<omega>)"
-| evs_and [simp]: "eval_stack \<Pi> (Bool i1 # Bool i2 # \<sigma>, \<phi>, And # \<pi>, s, \<omega>) 
-    (Bool (i2 \<and> i1) # \<sigma>, \<phi>, \<pi>, s, \<omega>)"
-| evs_or [simp]: "eval_stack \<Pi> (Bool i1 # Bool i2 # \<sigma>, \<phi>, Or # \<pi>, s, \<omega>) 
-    (Bool (i2 \<or> i1) # \<sigma>, \<phi>, \<pi>, s, \<omega>)"
-| evs_not [simp]: "eval_stack \<Pi> (Bool i1 # \<sigma>, \<phi>, Not # \<pi>, s, \<omega>) (Bool (\<not> i1) # \<sigma>, \<phi>, \<pi>, s, \<omega>)"
-| evs_push_c [simp]: "eval_stack \<Pi> (\<sigma>, \<phi>, Push (Constant i) # \<pi>, s, \<omega>) (IntV i # \<sigma>, \<phi>, \<pi>, s, \<omega>)"
+  evs_jump [simp]: "\<Pi> (frame.name f) = Some def \<Longrightarrow> stack_function_def.other_code def s = Some \<pi> \<Longrightarrow> 
+    eval_stack \<Pi> ([], f # \<phi>, ([], s), \<omega>) ([], f # \<phi>, \<pi>, \<omega>)"
+| evs_add [simp]: "eval_stack \<Pi> (IntV i1 # IntV i2 # \<sigma>, \<phi>, (Add # \<pi>, s), \<omega>) 
+    (IntV (i1 + i2) # \<sigma>, \<phi>, (\<pi>, s), \<omega>)"
+| evs_sub [simp]: "eval_stack \<Pi> (IntV i1 # IntV i2 # \<sigma>, \<phi>, (Sub # \<pi>, s), \<omega>) 
+    (IntV (i2 - i1) # \<sigma>, \<phi>, (\<pi>, s), \<omega>)"
+| evs_neg [simp]: "eval_stack \<Pi> (IntV i1 # \<sigma>, \<phi>, (Neg # \<pi>, s), \<omega>) (IntV (-i1) # \<sigma>, \<phi>, (\<pi>, s), \<omega>)"
+| evs_eq [simp]: "eval_stack \<Pi> (IntV i1 # IntV i2 # \<sigma>, \<phi>, (Eq # \<pi>, s), \<omega>) 
+    (Bool (i2 = i1) # \<sigma>, \<phi>, (\<pi>, s), \<omega>)"
+| evs_gt [simp]: "eval_stack \<Pi> (IntV i1 # IntV i2 # \<sigma>, \<phi>, (Gt # \<pi>, s), \<omega>) 
+    (Bool (i2 > i1) # \<sigma>, \<phi>, (\<pi>, s), \<omega>)"
+| evs_lt [simp]: "eval_stack \<Pi> (IntV i1 # IntV i2 # \<sigma>, \<phi>, (Lt # \<pi>, s), \<omega>) 
+    (Bool (i2 < i1) # \<sigma>, \<phi>, (\<pi>, s), \<omega>)"
+| evs_and [simp]: "eval_stack \<Pi> (Bool i1 # Bool i2 # \<sigma>, \<phi>, (And # \<pi>, s), \<omega>) 
+    (Bool (i2 \<and> i1) # \<sigma>, \<phi>, (\<pi>, s), \<omega>)"
+| evs_or [simp]: "eval_stack \<Pi> (Bool i1 # Bool i2 # \<sigma>, \<phi>, (Or # \<pi>, s), \<omega>) 
+    (Bool (i2 \<or> i1) # \<sigma>, \<phi>, (\<pi>, s), \<omega>)"
+| evs_not [simp]: "eval_stack \<Pi> (Bool i1 # \<sigma>, \<phi>, (Not # \<pi>, s), \<omega>) (Bool (\<not> i1) # \<sigma>, \<phi>, (\<pi>, s), \<omega>)"
+| evs_push_c [simp]: "eval_stack \<Pi> (\<sigma>, \<phi>, (Push (Constant i) # \<pi>, s), \<omega>) (IntV i # \<sigma>, \<phi>, (\<pi>, s), \<omega>)"
 | evs_push_l [simp]: "n < length (frame.locals f) \<Longrightarrow> 
-    eval_stack \<Pi> (\<sigma>, f # \<phi>, Push (Local n) # \<pi>, s, \<omega>) (frame.locals f ! n # \<sigma>, f # \<phi>, \<pi>, s, \<omega>)"
+    eval_stack \<Pi> (\<sigma>, f # \<phi>, (Push (Local n) # \<pi>, s), \<omega>) (frame.locals f ! n # \<sigma>, f # \<phi>, (\<pi>, s), \<omega>)"
 | evs_push_a [simp]: "n < length (frame.arguments f) \<Longrightarrow> 
-    eval_stack \<Pi> (\<sigma>, f # \<phi>, Push (Argument n) # \<pi>, s, \<omega>) (frame.arguments f ! n # \<sigma>, f# \<phi>, \<pi>, s, \<omega>)"
+    eval_stack \<Pi> (\<sigma>, f # \<phi>, (Push (Argument n) # \<pi>, s), \<omega>) 
+      (frame.arguments f ! n # \<sigma>, f # \<phi>, (\<pi>, s), \<omega>)"
 | evs_pop_l [simp]: "n < length (frame.locals f) \<Longrightarrow> 
-    eval_stack \<Pi> (v # \<sigma>, f # \<phi>, Pop (Local n) # \<pi>, s, \<omega>) 
-      (\<sigma>, f \<lparr> locals := frame.locals f [n := v] \<rparr> # \<phi>, \<pi>, s, \<omega>)"
+    eval_stack \<Pi> (v # \<sigma>, f # \<phi>, (Pop (Local n) # \<pi>, s), \<omega>) 
+      (\<sigma>, f \<lparr> locals := frame.locals f [n := v] \<rparr> # \<phi>, (\<pi>, s), \<omega>)"
 | evs_pop_a [simp]: "n < length (frame.arguments f) \<Longrightarrow> 
-    eval_stack \<Pi> (v # \<sigma>, f # \<phi>, Pop (Argument n) # \<pi>, s, \<omega>) 
-      (\<sigma>, f \<lparr> arguments := frame.arguments f [n := v] \<rparr> # \<phi>, \<pi>, s, \<omega>)"
-| evs_if_t [simp]: "eval_stack \<Pi> (Bool True # \<sigma>, \<phi>, IfJ \<pi>\<^sub>t \<pi>\<^sub>f # \<pi>, s, \<omega>) (\<sigma>, \<phi>, \<pi>\<^sub>t @ \<pi>, s, \<omega>)"
-| evs_if_f [simp]: "eval_stack \<Pi> (Bool False # \<sigma>, \<phi>, IfJ \<pi>\<^sub>t \<pi>\<^sub>f # \<pi>, s, \<omega>) (\<sigma>, \<phi>, \<pi>\<^sub>f @ \<pi>, s, \<omega>)"
-| evs_goto [simp]: "\<Pi> (frame.name f) = Some (a, l, \<pi>'', \<Phi>) \<Longrightarrow> \<Phi> s = Some (\<pi>', s') \<Longrightarrow> 
-    eval_stack \<Pi> ([], f # \<phi>, Goto s # \<pi>, s'', \<omega>) ([], f # \<phi>, \<pi>', s', \<omega>)"
-| evs_call [simp]: "\<Pi> f = Some (a, l, \<pi>, \<Phi>) \<Longrightarrow> length \<sigma> \<ge> a \<Longrightarrow> 
-    eval_stack \<Pi> (\<sigma>, \<phi>, Call f # \<pi>', s, \<omega>) ([], \<lparr> name = f, arguments = take a \<sigma>, locals = repeat (IntV 0) l, saved_stack = (drop a \<sigma>) \<rparr> # \<phi>, \<pi> @ \<pi>', s, \<omega>)"
+    eval_stack \<Pi> (v # \<sigma>, f # \<phi>, (Pop (Argument n) # \<pi>, s), \<omega>) 
+      (\<sigma>, f \<lparr> arguments := frame.arguments f [n := v] \<rparr> # \<phi>, (\<pi>, s), \<omega>)"
+| evs_if_t [simp]: "eval_stack \<Pi> (Bool True # \<sigma>, \<phi>, (IfJ \<pi>\<^sub>t \<pi>\<^sub>f # \<pi>, s), \<omega>) (\<sigma>, \<phi>, (\<pi>\<^sub>t @ \<pi>, s), \<omega>)"
+| evs_if_f [simp]: "eval_stack \<Pi> (Bool False # \<sigma>, \<phi>, (IfJ \<pi>\<^sub>t \<pi>\<^sub>f # \<pi>, s), \<omega>) (\<sigma>, \<phi>, (\<pi>\<^sub>f @ \<pi>, s), \<omega>)"
+| evs_goto [simp]: "\<Pi> (frame.name f) = Some def \<Longrightarrow> stack_function_def.other_code def s = Some \<pi>' \<Longrightarrow> 
+    eval_stack \<Pi> ([], f # \<phi>, (Goto s # \<pi>, _), \<omega>) ([], f # \<phi>, \<pi>', \<omega>)"
+| evs_call [simp]: "\<Pi> f = Some def \<Longrightarrow> length \<sigma> \<ge> stack_function_def.arity def \<Longrightarrow> 
+    eval_stack \<Pi> (\<sigma>, \<phi>, (Call f # \<pi>', s), \<omega>) ([], \<lparr> name = f, arguments = take a \<sigma>, 
+      locals = repeat (IntV 0) l, saved_stack = (drop a \<sigma>), saved_code = (\<pi>', s) \<rparr> # \<phi>, \<pi>, s', \<omega>)"
+
+
+(*
+
+
 | evs_return [simp]: "eval_stack \<Pi> (v # [], f # \<phi>, Return # \<pi>, s, \<omega>) 
-    (v # frame.saved_stack f, \<phi>, \<pi>, s, \<omega>)"
+    (v # frame.saved_stack f, \<phi>, fst (frame.saved_code f), snd (frame.saved_code f), \<omega>)"
 | evs_print [simp]: "eval_stack \<Pi> (IntV i1 # \<sigma>, \<phi>, Print # \<pi>, s, \<omega>) (\<sigma>, \<phi>, \<pi>, s, i1 # \<omega>)"
+*)
 
 fun stack_output :: "stack_state \<Rightarrow> output" where
-  "stack_output (\<sigma>, \<phi>, \<pi>, s, \<omega>) = \<omega>"
+  "stack_output (\<sigma>, \<phi>, \<pi>, \<omega>) = \<omega>"
 
 (* state validity *)
 
 fun valid_frame :: "stack_program \<Rightarrow> frame \<Rightarrow> bool" where
-  "valid_frame \<Pi> \<lparr> name = f, arguments = as, locals = ls, saved_stack = \<sigma> \<rparr> = (case \<Pi> f of
-      Some (a, l, \<Phi>) \<Rightarrow> length as = a \<and> length ls = l
-    | None \<Rightarrow> False)"
+  "valid_frame \<Pi> \<lparr> name = f, arguments = as, locals = ls, saved_stack = \<sigma>, saved_code = \<pi> \<rparr> = (
+    case \<Pi> f of
+        Some def \<Rightarrow> length as = stack_function_def.arity def \<and> 
+          length ls = stack_function_def.local_count def
+      | None \<Rightarrow> False)"
 
 fun valid_state :: "stack_program \<Rightarrow> stack_state \<Rightarrow> bool" where
-  "valid_state \<Pi> (\<sigma>, \<phi>, \<pi>, s, \<omega>) = (\<forall>f \<in> set \<phi>. valid_frame \<Pi> f)"
+  "valid_state \<Pi> (\<sigma>, \<phi>, \<pi>, \<omega>) = (\<forall>f \<in> set \<phi>. valid_frame \<Pi> f)"
 
 lemma [simp]: "valid_frame \<Pi> fr \<Longrightarrow> valid_frame \<Pi> (fr\<lparr>locals := locals fr[n := v]\<rparr>)"
   by (cases fr) (auto split: option.splits)
@@ -93,8 +109,8 @@ lemma [simp]: "valid_frame \<Pi> fr \<Longrightarrow> valid_frame \<Pi> (fr\<lpa
 lemma [simp]: "valid_frame \<Pi> fr \<Longrightarrow> valid_frame \<Pi> (fr\<lparr>arguments := arguments fr[n := v]\<rparr>)"
   by (cases fr) (auto split: option.splits)
 
-lemma [simp]: "valid_frame \<Pi> fr \<Longrightarrow> \<Pi> (frame.name fr) = Some (a, l, \<Phi>) \<Longrightarrow> 
-    length (frame.locals fr) = l"
+lemma [simp]: "valid_frame \<Pi> fr \<Longrightarrow> \<Pi> (frame.name fr) = Some def \<Longrightarrow> 
+    length (frame.locals fr) = stack_function_def.local_count def"
   by (cases fr) simp
 
 lemma [simp]: "eval_stack \<Pi> \<Sigma> \<Sigma>' \<Longrightarrow> valid_state \<Pi> \<Sigma> \<Longrightarrow> valid_state \<Pi> \<Sigma>'"
